

Review - Course Pack - Page 31

1

$$1a) \lim_{x \rightarrow -4} \frac{x^2 + 5x + 4}{x^2 + 3x - 4}$$

$$= \lim_{x \rightarrow -4} \frac{\cancel{(x+4)}(x+1)}{\cancel{(x+4)}(x-1)}$$

$$= \frac{3}{5}$$

$$b) \lim_{x \rightarrow 3} \frac{2x^2 - x - 15}{3x^2 - 13x + 12}$$

$$= \lim_{x \rightarrow 3} \frac{(2x+5)\cancel{(x-3)}}{(3x-4)\cancel{(x-3)}}$$

$$= \lim_{x \rightarrow 3} \frac{2x+5}{3x-4}$$

$$= \frac{11}{5}$$

$$c) \lim_{x \rightarrow -4} \frac{\sqrt{x^2+9} - 5}{x+4}$$

$$= \lim_{x \rightarrow -4} \frac{(\sqrt{x^2+9} - 5)(\sqrt{x^2+9} + 5)}{(x+4)(\sqrt{x^2+9} + 5)}$$

$$= \lim_{x \rightarrow -4} \frac{x^2 + 9 - 25}{(x+4)(\sqrt{x^2+9} + 5)}$$

$$= \lim_{x \rightarrow -4} \frac{\cancel{(x+4)}(x-4)}{\cancel{(x+4)}(\sqrt{x^2+9} + 5)}$$

$$= \frac{-8}{10}$$

$$= \frac{-4}{5}$$

$$d) \lim_{x \rightarrow 16} \frac{4 - \sqrt{x}}{16x - x^2}$$

$$= \lim_{x \rightarrow 16} \frac{(4 - \sqrt{x})(4 + \sqrt{x})}{16x - x^2} \frac{(4 + \sqrt{x})}{(4 + \sqrt{x})}$$

$$= \lim_{x \rightarrow 16} \frac{\cancel{16-x}}{x(\cancel{16-x})(4 + \sqrt{x})}$$

$$= \frac{1}{128}$$

(2)

$$\begin{aligned}
 \text{e) } \lim_{x \rightarrow -4} \frac{\frac{1}{4} + \frac{1}{x}}{4+x} \\
 = \lim_{x \rightarrow -4} \frac{\cancel{x+4}}{4x(\cancel{4+x})} \\
 = \frac{-1}{16}
 \end{aligned}$$

$$\begin{aligned}
 \text{f) } \lim_{x \rightarrow 4} \frac{x^3 - 64}{x - 4} \\
 = \lim_{x \rightarrow 4} \frac{(x-4)(x^2 + 4x + 16)}{\cancel{x-4}} \\
 = 48
 \end{aligned}$$

$$\text{g) } \lim_{x \rightarrow -\infty} \frac{-2x^3 + 5x - 7}{x^2 + 5x + 4}$$

$$\begin{aligned}
 = \lim_{x \rightarrow -\infty} \frac{-2x^3}{x^2} + \lim_{x \rightarrow -\infty} \frac{5x}{x^2} - \lim_{x \rightarrow -\infty} \frac{7}{x^2} \\
 \lim_{x \rightarrow -\infty} \frac{x^2}{x^2} + 5 \lim_{x \rightarrow -\infty} \frac{x}{x^2} + \lim_{x \rightarrow -\infty} \frac{4}{x^2}
 \end{aligned}$$

$$\begin{aligned}
 = \lim_{x \rightarrow -\infty} \frac{-2x}{1} + \lim_{x \rightarrow -\infty} \frac{5}{x} - \lim_{x \rightarrow -\infty} \frac{7}{x^2} \\
 = \frac{\infty + 0 - 0}{1 + 0 + 0} = \infty
 \end{aligned}$$

$$\begin{aligned}
 \text{h) } \lim_{x \rightarrow \infty} \frac{2x^3 - 1}{5x^3 + 2x^2 - 3x} \\
 = \lim_{x \rightarrow \infty} \frac{2x^3}{x^3} - \lim_{x \rightarrow \infty} \frac{1}{x^3} \\
 \frac{5 \lim_{x \rightarrow \infty} \frac{x^3}{x^3} + 2 \lim_{x \rightarrow \infty} \frac{x^2}{x^3} - 3 \lim_{x \rightarrow \infty} \frac{x}{x^3}}{5 \lim_{x \rightarrow \infty} 1 + 2 \lim_{x \rightarrow \infty} \frac{1}{x} - 3 \lim_{x \rightarrow \infty} \frac{1}{x}} \\
 = \frac{2 - 0}{5 + 0 - 0} = \frac{2}{5}
 \end{aligned}$$

(2)

$$e) \lim_{x \rightarrow -4} \frac{\frac{1}{4} + \frac{1}{x}}{4+x}$$

$$= \lim_{x \rightarrow -4} \frac{\cancel{x+4}}{4x(\cancel{4+x})}$$

$$= -\frac{1}{16}$$

$$h) \lim_{x \rightarrow \infty} \frac{2x^3 - 1}{5x^3 + 2x^2 - 3x}$$

$$= \lim_{x \rightarrow \infty} \frac{2x^3}{x^3} - \lim_{x \rightarrow \infty} \frac{1}{x^3}$$

$$5 \lim_{x \rightarrow \infty} \frac{x^3}{x^3} + 2 \lim_{x \rightarrow \infty} \frac{x^2}{x^3} - 3 \lim_{x \rightarrow \infty} \frac{x}{x^3}$$

$$= \lim_{x \rightarrow \infty} 2 - \lim_{x \rightarrow \infty} \frac{1}{x^3}$$

$$5 \lim_{x \rightarrow \infty} 1 + 2 \lim_{x \rightarrow \infty} \frac{1}{x} - 3 \lim_{x \rightarrow \infty} \frac{1}{x}$$

$$= \frac{2-0}{5+0-0} = \frac{2}{5}$$

$$f) \lim_{x \rightarrow 4} \frac{x^3 - 64}{x - 4}$$

$$= \lim_{x \rightarrow 4} \frac{(x-4)(x^2 + 4x + 16)}{\cancel{x-4}}$$

$$= 48$$

$$g) \lim_{x \rightarrow -\infty} \frac{-2x^3 + 5x - 7}{x^2 + 5x + 4}$$

$$= \lim_{x \rightarrow -\infty} \frac{-2x^3}{x^2} + \lim_{x \rightarrow -\infty} \frac{5x}{x^2} - \lim_{x \rightarrow -\infty} \frac{7}{x^2}$$

$$\lim_{x \rightarrow -\infty} \frac{x^2}{x^2} + 5 \lim_{x \rightarrow -\infty} \frac{x}{x^2} + \lim_{x \rightarrow -\infty} \frac{4}{x^2}$$

$$= \lim_{x \rightarrow -\infty} -2x + \lim_{x \rightarrow -\infty} \frac{5}{x} - \lim_{x \rightarrow -\infty} \frac{7}{x^2} = \frac{\infty + 0 - 0}{1 + 0 + 0} = \infty$$

$$\lim_{x \rightarrow -\infty} 1 + 5 \lim_{x \rightarrow -\infty} \frac{1}{x} + \lim_{x \rightarrow -\infty} \frac{4}{x^2}$$

(3)

$$2a) f(x) = 2x^2 - 3x$$

$$f'(x) = \lim_{h \rightarrow 0} \frac{f(x+h) - f(x)}{h}$$

$$= \lim_{h \rightarrow 0} \frac{2(x+h)^2 - 3(x+h) - (2x^2 - 3x)}{h}$$

$$= \lim_{h \rightarrow 0} \frac{2(x^2 + 2xh + h^2) - 3x - 3h - 2x^2 + 3x}{h}$$

$$= \lim_{h \rightarrow 0} \frac{4xh + 2h^2 - 3h}{h}$$

$$= 4x - 3$$

$$b) f(x) = \frac{1}{3x+2}$$

$$f'(x) = \lim_{h \rightarrow 0} \frac{f(x+h) - f(x)}{h}$$

$$= \lim_{h \rightarrow 0} \frac{\frac{1}{3(x+h)+2} - \frac{1}{3x+2}}{h}$$

$$= \lim_{h \rightarrow 0} \frac{3x+2 - (3(x+h)+2)}{h(3(x+h)+2)(3x+2)}$$

$$= \lim_{h \rightarrow 0} \frac{\cancel{3x+2} - \cancel{3x} - 3h - \cancel{2}}{h(\cancel{3x+3h+2})(3x+2)}$$

$$= \frac{-3}{(3x+2)^2}$$

$$3. y = x^2 - 6x + 9$$

$$y' = \lim_{h \rightarrow 0} \frac{f(x+h) - f(x)}{h}$$

$$= \lim_{h \rightarrow 0} \frac{(x+h)^2 - 6(x+h) + 9 - (x^2 - 6x + 9)}{h}$$

$$= \lim_{h \rightarrow 0} \frac{\cancel{x^2} + 2xh + \cancel{h^2} - \cancel{6x} - 6h + \cancel{9} - \cancel{x^2} + \cancel{6x} - \cancel{9}}{h}$$

$$= \lim_{h \rightarrow 0} \frac{2xh + h^2 - 6h}{h}$$

$$= 2x - 6$$

$$\therefore m_t|_{x=2} = -2 \Rightarrow y - 1 = -2(x - 2)$$

$$\therefore m_{\perp}|_{x=2} = \frac{1}{2} \Rightarrow y - 1 = \frac{1}{2}(x - 2)$$

$$4. y = x^2 - 5x + 4$$

$$y' = \lim_{h \rightarrow 0} \frac{f(x+h) - f(x)}{h}$$

$$= \lim_{h \rightarrow 0} \frac{(x+h)^2 - 5(x+h) + 4 - (x^2 - 5x + 4)}{h}$$

$$= \lim_{h \rightarrow 0} \frac{\cancel{x^2} + 2xh + \cancel{h^2} - \cancel{5x} - 5h + \cancel{4} - \cancel{x^2} + \cancel{5x} - \cancel{4}}{h}$$

$$= \lim_{h \rightarrow 0} \frac{2xh + h^2 - 5h}{h}$$

$$\perp \text{ to } y = -\frac{1}{3}x + 5$$

$$\Rightarrow m_t = 3$$

$$= 2x - 5$$

$$\therefore 2x - 5 = 3$$

$$x = 4$$

$$\therefore y = 3(x - 4)$$

$$\begin{aligned}
 5. a) \text{ AROC} &= \frac{h(t_2) - h(t_1)}{t_2 - t_1} \\
 &= \frac{\cancel{500} - 5(3)^2 - (\cancel{500} - 5(1)^2)}{3 - 1} \\
 &= \frac{-45 + 5}{2} \\
 &= -20 \text{ m/s.}
 \end{aligned}$$

b) Evaluate $\lim_{a \rightarrow 2} \frac{h(t+a) - h(t)}{a}$.

Answer is -20 m/s.

$$6. f(x) = \begin{cases} -2x - 8 & x \leq -2 \\ \frac{3}{2}x - 1 & -2 < x \leq 2 \\ (x-4)^2 - 6 & x > 2 \end{cases}$$

At $x = -2$

$$\textcircled{1} f(-2) = -4$$

$$\textcircled{2} \lim_{x \rightarrow -2^-} f(x)$$

$$= \lim_{x \rightarrow -2^-} -2x - 8$$

$$= -4$$

$$\Rightarrow \lim_{x \rightarrow -2} f(x) = -4$$

$$= \lim_{x \rightarrow -2^+} \frac{3}{2}x - 1$$

$$= -4$$

$$\textcircled{3} f(-2) = \lim_{x \rightarrow -2} f(x)$$

* \therefore cont. @ $x = -2$

At $x = 2$

$$\textcircled{1} f(2) = 1$$

$$\textcircled{2} \lim_{x \rightarrow 2^-} f(x)$$

$$= \lim_{x \rightarrow 2^-} \frac{3}{2}x - 1$$

$$= 1$$

$$\Rightarrow \lim_{x \rightarrow 2} f(x) \text{ DNE.}$$

$$= \lim_{x \rightarrow 2^+} (x-4)^2 - 6$$

$$= -2$$

* \therefore Not cont. @ $x = 2$